WIP

theories/Hoare.v
@@ -15,6 +15,20 @@ Set Implicit Arguments.
 
 
 
+Section AUX________REMOVEME_____REDUNDANT.
+
+  Context `{Σ: GRA.t}.
+
+  Definition refines_closed (md_tgt md_src: ModL.t): Prop :=
+    Beh.of_program (ModL.compile md_tgt) <1= Beh.of_program (ModL.compile md_src)
+  .
+
+  Global Program Instance refines_closed_PreOrder: PreOrder refines_closed.
+  Next Obligation. ii; ss. Qed.
+  Next Obligation. ii; ss. r in H. r in H0. eauto. Qed.
+
+End AUX________REMOVEME_____REDUNDANT.
+
 
 
 Section CANCEL.
@@ -46,9 +60,138 @@ Section CANCEL.
   Hypothesis MAINPRE: main_pre ([]: list val)↑ ord_top entry_r.
   Hypothesis WFR: URA.wf (entry_r ⋅ rsum (ModSemL.initial_r_state ms_tgt)).
 
-  Theorem adequacy_type: Beh.of_program (ModL.compile md_tgt) <1= Beh.of_program (ModL.compile md_src).
+  Theorem adequacy_type: refines_closed md_tgt md_src.
   Proof.
     ii. eapply adequacy_type_m2s. eapply adequacy_type_t2m; et.
   Qed.
 
 End CANCEL.
+
+
+
+
+Section AUX.
+
+  Context `{Σ: GRA.t}.
+
+  Lemma modl_eta: forall x0 x1 y0 y1, x0 = x1 -> y0 = y1 -> (ModL.mk x0 y0) = (ModL.mk x1 y1).
+  Proof. i; subst. refl. Qed.
+
+  Lemma modseml_eta: forall x0 x1 y0 y1, x0 = x1 -> y0 = y1 -> (ModSemL.mk x0 y0) = (ModSemL.mk x1 y1).
+  Proof. i; subst. refl. Qed.
+
+End AUX.
+
+
+Lemma sk_unit_id: forall sk, (Sk.add sk Sk.unit) = sk.
+Proof. i. unfold Sk.add, Sk.unit. rewrite app_nil_r. refl. Qed.
+
+Lemma sk_unit_idl: forall sk, (Sk.add Sk.unit sk) = sk.
+Proof. i. unfold Sk.add, Sk.unit. rewrite app_nil_l. refl. Qed.
+
+
+
+
+
+
+Section BETTER.
+
+  Context `{Σ: GRA.t}.
+
+  Variable mds: list SMod.t.
+
+  Let sk: Sk.t := fold_right Sk.add Sk.unit (List.map SMod.sk mds).
+  Let skenv: SkEnv.t := Sk.load_skenv sk.
+  Let mss: list SModSem.t := (List.map ((flip SMod.get_modsem) skenv) mds).
+  (* Let stb: list (gname * fspec) := List.concat (List.map (List.map (fun '(fn, fs) => (fn, fsb_fspec fs)) ∘ SModSem.fnsems) mss). *)
+  Let sbtb: list (gname * fspecbody) := (List.flat_map (SModSem.fnsems) mss).
+  (* Let stb: list (gname * fspec) := (List.flat_map (List.map (fun '(fn, fs) => (fn, fsb_fspec fs)) ∘ SModSem.fnsems) mss). *)
+  Let stb: list (gname * fspec) := List.map (fun '(fn, fs) => (fn, fs.(fsb_fspec))) sbtb.
+
+  Let mds_src: list Mod.t := List.map (SMod.to_src) mds.
+  Let mds_tgt: list Mod.t := List.map (SMod.to_tgt stb) mds.
+
+  (* Let rsum: r_state -> Σ := *)
+  (*   fun '(mrs_tgt, frs_tgt) => (URA.add (fold_left URA.add (List.map (mrs_tgt <*> fst) ms_tgt.(ModSemL.initial_mrs)) ε) *)
+  (*                                       (fold_left URA.add frs_tgt ε)). *)
+
+  Variable entry_r: Σ.
+  Variable main_pre: Any.t -> ord -> Σ -> Prop.
+  Hypothesis MAIN: List.find (fun '(_fn, _) => dec "main" _fn) stb =
+                   Some ("main", (mk_simple "Main" (fun (_: unit) => (main_pre, top2)))).
+  Hypothesis MAINPRE: main_pre ([]: list val)↑ ord_top entry_r.
+  (* Hypothesis WFR: URA.wf (entry_r ⋅ fold_right (⋅) ε (List.map SModSem.initial_mr mss)). *)
+  Hypothesis WFR: URA.wf (entry_r ⋅ fold_left (⋅) (List.map SModSem.initial_mr mss) ε).
+
+  Theorem adequacy_type_better: refines_closed (Mod.add_list mds_tgt) (Mod.add_list mds_src).
+  Proof.
+    etrans.
+    { eapply adequacy_type; et.
+      - unfold mds_tgt. ss.
+        replace (Sk.load_skenv (ModL.sk (Mod.add_list (List.map (SMod.to_tgt stb) mds)))) with skenv; cycle 1.
+        { unfold skenv. f_equal. unfold sk. unfold Mod.add_list.
+          rewrite List.map_map. clear.
+          (* subst_locals. *)
+          induction mds; ii; ss.
+          rewrite IHl.
+          assert(U: forall x y z, x = y -> Sk.add z x = Sk.add z y).
+          { i; subst; refl. }
+          eapply U.
+          assert(V: forall x y, x = y -> ModL.sk x = ModL.sk y).
+          { i; subst; refl. }
+          eapply V.
+          assert(W: forall A B (s: A) (f: B -> A -> A) x y, x = y -> fold_right f s x = fold_right f s y).
+          { i; subst; refl. }
+          eapply W.
+          eapply map_ext. i. r.
+          replace (List.map (fun '(fn, fs) => (fn, fs.(fsb_fspec)))
+                            (flat_map SModSem.fnsems (List.map (flip SMod.get_modsem
+                                      (Sk.load_skenv (fold_right Sk.add Sk.unit (List.map SMod.sk l)))) l))) with stb.
+          { refl. }
+          unfold stb. unfold sbtb.
+          clear.
+          rewrite ! flat_map_concat_map.
+          rewrite concat_map.
+          eapply map_ext.
+          f_equal.
+          (* Set Ltac Profiling. Show Ltac Profile. *)
+          f_equal.
+          destruct mds; ss. clear mds.
+          destruct l; ss.
+          destruct l; ss.
+          destruct l; ss.
+          {
+          admit "somehow".
+        }
+        unfold Mod.add_list. unfold Mod.lift.
+        admit "somehow?".
+      - des_ifs. ss. erewrite f_equal; [apply WFR|]. repeat f_equal.
+        unfold ModSemL.initial_r_state in Heq. clarify. ss. repeat rewrite URA.unit_id. f_equal.
+        admit "somehow?".
+    }
+    erewrite f_equal.
+    { refl. }
+    unfold md_src, mds_src.
+    clear. subst_locals.
+    destruct mds; ss.
+    destruct l; ss.
+    { rewrite List.app_nil_r. rewrite ! Mod.add_list_single.
+      destruct t; ss. cbn. unfold SMod.to_src. ss.
+      eapply modl_eta; ss; cycle 1.
+      { admit "". }
+      apply func_ext. i. unfold ms_src. ss.
+      assert(x = Sk.load_skenv sk) by admit "". subst.
+      unfold SModSem.to_src. eapply modseml_eta; ss; cycle 1.
+      unfold ModSem.map_snd. unfold compose.
+      rewrite sk_unit_id.
+      set (skenv:=(Sk.load_skenv sk)).
+      rewrite List.map_map. f_equal.
+      apply func_ext. i. des_ifs. f_equal.
+      assert(T: mn f = (SModSem.mn (get_modsem skenv))).
+      { admit "mn condition". }
+      rewrite T. refl.
+    }
+    admit "".
+  Qed.
+
+End BETTER.
